pure_model/mul_error.lean
@@ -1,0 +1,121 @@
+
+import LeanRV64DLEAN.Sail.Sail
+import LeanRV64DLEAN.Sail.BitVec
+import LeanRV64DLEAN.Defs
+import LeanRV64DLEAN.Specialization
+import LeanRV64DLEAN.RiscvExtras
+import LeanRV64DLEAN
+
+
+open Functions
+open Retired
+open Sail
+
+
+/- MUL function from the SailLean modell
+
+def execute_MUL (rs2 : regidx) (rs1 : regidx) (rd : regidx) (mul_op : mul_op) : SailM Retired := do
+  let rs1_val ← do (rX_bits rs1)
+  let rs2_val ← do (rX_bits rs2)
+  let rs1_int : Int :=
+    if mul_op.signed_rs1
+    then (BitVec.toInt rs1_val)
+    else (BitVec.toNat rs1_val)
+  let rs2_int : Int :=
+    if mul_op.signed_rs2
+    then (BitVec.toInt rs2_val)
+    else (BitVec.toNat rs2_val)
+  let result_wide := (to_bits (2 *i xlen) (rs1_int *i rs2_int))
+  let result :=
+    if mul_op.high
+    then (Sail.BitVec.extractLsb result_wide ((2 *i xlen) -i 1) xlen)
+    else (Sail.BitVec.extractLsb result_wide (xlen -i 1) 0)
+  (wX_bits rd result)
+  (pure RETIRE_SUCCESS)
+-/
+
+/-
+
+
+/-- Type quantifiers: n : Int, l : Nat, l ≥ 0 -/
+def to_bits (l : Nat) (n : Int) : (BitVec l) :=
+  (get_slice_int l n 0)
+
+
+def get_slice_int (len lo : Nat) (n : Int) : BitVec len :=
+  BitVec.extractLsb' lo len (BitVec.ofInt (lo + len + 1) n)
+
+def to_bits (l : Nat) (n : Int) : (BitVec l) :=
+  (get_slice_int l n 0)
+
+
+-- Sail version
+def extractLsb {w : Nat} (x : BitVec w) (hi lo : Nat) : BitVec (hi - lo + 1) :=
+  x.extractLsb hi lo
+
+-/
+def get_slice_int1 (len lo : Nat) (n : Int) : BitVec len :=
+  BitVec.extractLsb' lo len (BitVec.ofInt (lo + len + 1) n)
+
+
+def execute_MUL_pure64 (mul_op : mul_op) (rs2_val : (BitVec 64)) (rs1_val : (BitVec 64)) : BitVec 64 :=
+  let rs1_int : Int :=
+    if mul_op.signed_rs1 -- if signed then modell as integer operation
+    then (BitVec.toInt rs1_val)
+    else (BitVec.toNat rs1_val)
+    --dbg_trace " hello {rs1_val.toInt}"
+  let rs2_int : Int :=
+    if mul_op.signed_rs2
+    then (BitVec.toInt rs2_val)
+    else (BitVec.toNat rs2_val)
+  dbg_trace " START  {rs1_int} {rs2_int} {rs1_int *i rs2_int }"
+  let result_wide := (get_slice_int1 (2 *i Functions.xlen) 0 (rs1_int *i rs2_int) ) --adapt result vector width to 2^(exp1 + exp2)
+  dbg_trace " AFTER {result_wide}"
+  dbg_trace " len {2 *i Functions.xlen}"
+  let result :=
+    if mul_op.high -- if set return the higher xlen bits else the lower
+    then (Sail.BitVec.extractLsb result_wide ((2 *i Functions.xlen) -i 1) Functions.xlen) --return either higher or lower xlen bits
+    else (Sail.BitVec.extractLsb result_wide (Functions.xlen -i 1) 0)
+  result
+
+def skeleton_binary  (rs2 : regidx) (rs1 : regidx) (rd : regidx) (execute_func : BitVec 64 → BitVec 64 → BitVec 64) : SailM Retired := do
+  let rs1_val ← rX_bits rs1
+  let rs2_val ← rX_bits rs2
+  let result := execute_func rs1_val rs2_val
+  wX_bits rd result
+  pure RETIRE_SUCCESS
+
+
+theorem mul_eq (rs2 : regidx) (rs1 : regidx) (rd : regidx) (mul_op : mul_op) :
+    Functions.execute_MUL (rs2 ) (rs1) (rd) (mul_op)
+      = skeleton_binary rs2 rs1 rd (fun val1 val2 => execute_MUL_pure64 mul_op val2 val1)
+  := by
+  unfold Functions.execute_MUL skeleton_binary execute_MUL_pure64
+  rfl
+
+
+
+def x := BitVec.ofInt 64 (-1)
+
+/- this file was for debugging the riscv semantics of the saillean modell -/
+#eval  execute_MUL_pure64 (mul_op := { high := False, signed_rs1:= False, signed_rs2 := False }) (10#64) (9#64)
+
+#eval  execute_MUL_pure64 (mul_op := { high := False, signed_rs1:= True, signed_rs2 := False }) (100#64) (x)
+
+
+example : execute_MUL_pure64 (mul_op := { high := False, signed_rs1:= False, signed_rs2 := False }) (1#64) (1#64)
+  = 1#64 := rfl
+
+
+#eval  execute_MUL_pure64 (mul_op := { high := False, signed_rs1:= False, signed_rs2 := False }) (9#64) (99#64)
+
+
+
+/-
+example :
+  let mul_op := { high := False, signed_rs1:= False, signed_rs2 := False }
+  let state := sorry
+  let r0 := regidx.Regidx 0#5
+  Functions.execute_MUL r0 r0 r0 mul_op state
+  = ...
+-/
